agree/agree_fullSyntax.sml
@@ -1,0 +1,88 @@
+structure agree_fullSyntax :> agree_fullSyntax =
+struct
+
+local open agree_fullTheory in end
+
+open HolKernel boolLib;
+
+val expr_ty = mk_thy_type{Thy="agree_full", Tyop = "expr", Args = []};
+val component_ty = mk_thy_type{Thy="agree_full", Tyop="component", Args=[]};
+
+(*---------------------------------------------------------------------------*)
+(* Expressions                                                               *)
+(*---------------------------------------------------------------------------*)
+
+fun agree_const s = prim_mk_const{Thy = "agree_full", Name = s};
+
+val Var_const = agree_const "VarExpr"
+val IntLit_const = agree_const "IntLit";
+val BoolLit_const = agree_const "BoolLit";
+val Not_const = agree_const "NotExpr";
+val Pre_const = agree_const "PreExpr";
+val Hist_const = agree_const "HistExpr";
+val Add_const = agree_const "AddExpr";
+val Sub_const = agree_const "SubExpr";
+val Mult_const = agree_const "MultExpr";
+val Div_const = agree_const "DivExpr";
+val Mod_const = agree_const "ModExpr";
+val Or_const = agree_const "OrExpr";
+val And_const = agree_const "AndExpr";
+val Imp_const = agree_const "ImpExpr";
+val Iff_const = agree_const "IffExpr";
+val Eq_const = agree_const "EqExpr";
+val Leq_const = agree_const "LeqExpr";
+val Lt_const = agree_const "LtExpr";
+val Recd_const = agree_const "RecdExpr";
+val RecdProj_const = agree_const "RecdProj";
+val Array_const = agree_const "ArrayExpr";
+val ArraySub_const = agree_const "ArraySub";
+val PortEvent_const = agree_const "PortEvent";
+val PortData_const = agree_const "PortData";
+val Fby_const = agree_const "FbyExpr";
+val Cond_const = agree_const "CondExpr";
+val eventOf_const = agree_const "eventOf";
+val dataOf_const = agree_const "dataOf";
+val component_const = agree_const "recordtype.component";
+val Stmt_const = agree_const "Stmt";
+val Output_Data_const = agree_const "Output_Data";
+val Output_Event_const = agree_const "Output_Event";
+val Output_Event_Data_const = agree_const "Output_Event_Data";
+
+
+val mk_Var = mk_monop Var_const
+val mk_IntLit = mk_monop IntLit_const
+val mk_BoolLit = mk_monop BoolLit_const
+val mk_Not = mk_monop Not_const
+val mk_Pre = mk_monop Pre_const
+val mk_Hist = mk_monop Hist_const
+val mk_Add = mk_binop Add_const
+val mk_Sub = mk_binop Sub_const
+val mk_Mult = mk_binop Mult_const
+val mk_Div = mk_binop Div_const
+val mk_Mod = mk_binop Mod_const
+val mk_Or = mk_binop Or_const
+val mk_And = mk_binop And_const
+val mk_Imp = mk_binop Imp_const
+val mk_Iff = mk_binop Iff_const
+val mk_Eq = mk_binop Eq_const
+val mk_Leq = mk_binop Leq_const
+val mk_Lt = mk_binop Lt_const
+
+val mk_RecdProj = mk_binop RecdProj_const
+val mk_ArraySub = mk_binop ArraySub_const
+val mk_PortEvent = mk_monop PortEvent_const
+val mk_PortData  = mk_monop PortData_const
+val mk_Fby = mk_binop Fby_const
+val mk_Cond = mk_triop Cond_const;
+
+val mk_Recd = mk_monop Recd_const
+val mk_Array = mk_monop Array_const;
+
+val mk_stmt = mk_binop Stmt_const;
+val mk_output_data = mk_binop Output_Data_const;
+val mk_output_event = mk_binop Output_Event_const;
+val mk_output_event_data = mk_triop Output_Event_Data_const;
+
+fun mk_component fields = TypeBase.mk_record(component_ty, fields)
+
+end
